\documentclass[12pt]{article}
\usepackage{amssymb, amsmath, amsfonts}
\usepackage{graphicx}
\usepackage{tabularx}
\usepackage{braket}
\usepackage{siunitx}

\newcommand{\ep}{\epsilon}

\begin{document}
\title{Cavity Spatial and Temporal Profile derivation}
\author{Justin Gerber}
\date{\today}
\maketitle

\section{Introduction}

In my thesis I have calculate the position and time dependent right and left propagating fields in an optical cavity.

\begin{align}
E_{cav,R}^{(+)}(z,t) =& E_{in,0}^{(+)}t_1\frac{\mathcal{F}}{\pi} \chi(\Delta) e^{-i(\psi(z)-\psi(z_1))}e^{ik_q(z-z_1)}e^{-i\omega_q t}\\
E_{cav,L}^{(+)}(z,t) =& -E_{in,0}^{(+)}r_2t_1\frac{\mathcal{F}}{\pi}\chi(\Delta) e^{+i(\psi(z)-\psi(z_2))}e^{-ik_q(z-z_2)} e^{+i\frac{\phi_{r_1} - \phi_{r_2}}{2}} e^{i\pi q} e^{-i\omega_q t}
\end{align}

A few notes

\begin{align}
\omega_{FSR} =& 2\pi \frac{c}{2L}\\
k_{FSR} =& \frac{\omega_{FSR}}{c} = \frac{\pi}{L}\\
\omega_q =& \omega_{FSR}\left(q + \frac{\phi_C}{2\pi}\right)\\
k_q =& k_{FSR}\left(q+\frac{\phi_C}{2\pi}\right) = \frac{\pi}{L}\left(q+\frac{\phi_C}{2\pi}\right)\\
\phi_C =& 2\phi_G + \phi_{r_1}+\phi_{r_2}\\
\phi_G =& \psi(z_2)-\psi(z_1)\\
L =& z_2 - z_1
\end{align}

We can write this as

\begin{align}
E_{cav,R}^{(+)}(z,t) =& E_{in,0}^{(+)}t_1\frac{\mathcal{F}}{\pi}\chi(\Delta) e^{i\Phi_{cav,R}}\\
E_{cav,L}^{(+)}(z,t) =& E_{in,0}^{(+)}t_1\frac{\mathcal{F}}{\pi}\chi(\Delta) e^{i\Phi_{cav,L}}
\end{align}

Where I have approximated $r_2\approx 1$ and defined

\begin{align}
\Phi_{cav,R} =& k_q(z-z_1) - (\psi(z)-\psi(z_1)) - \omega_q t\\
\Phi_{cav,L} =& -k_q(z-z_2) + (\psi(z)-\psi(z_2)) +\frac{\phi_{r_1}-\phi_{r_2}}{2} + \pi(q + 1) - \omega_q t
\end{align}

The extra term of $\pi$ in $\Phi_{cav,L}$ comes from $-1 = e^{+i\pi}$. 
The standing wave inside of the cavity is the sum of the left and right propagating fields:

\begin{align}
E_{cav}(z,t) =& E_{cav,R}^{(+)}(z,t) + E_{cav,L}^{(+)}(z,t) + c.c.\\
=& E_{in,0}^{(+)}t_1\frac{\mathcal{F}}{\pi}\chi(\Delta)\\
=& E_{in,0}^{(+)}t_1\frac{\mathcal{F}}{\pi}\chi(\Delta)\left(e^{i\Phi_{cav,R}} + e^{i\Phi_{cav,L}} + c.c.\right)
\end{align}

We have the identity

\begin{align}
e^A + e^B + e^{-A} + e^{-B} =& \left(e^{\frac{A+B}{2}} + e^{-\frac{A+B}{2}}\right)\left(e^{\frac{A-B}{2}} + e^{-\frac{A-B}{2}}\right)\\
\end{align}

From which we can derive the trig identity

\begin{align}
2(\cos(A) + \cos(B)) = 4\cos\left(\frac{A+B}{2}\right)\cos\left(\frac{A-B}{2}\right)
\end{align}

So we are interested in

\begin{align}
\Phi_+ =& \frac{1}{2}\left(\Phi_{cav,_R} + \Phi_{cav,L}\right)\\
\Phi_- =& \frac{1}{2}\left(\Phi_{cav,_R} - \Phi_{cav,L}\right)
\end{align}

\begin{align}
\Phi_+(t) =& -\omega_q t + \frac{1}{2}k_q(z_2-z_1) - \frac{1}{2}(\psi(z_2)-\psi(z_1)) + \frac{\phi_{r_1} - \phi_{r_2}}{4} + \frac{\pi}{2}(q+1)\\
=& -\omega_q t + \frac{\pi}{2}\left(q + \frac{\phi_C}{2\pi}\right) -\frac{\phi_G}{2} + \frac{\phi_{r_1} - \phi_{r_2}}{4} + \frac{\pi}{2}(q+1)\\
=& -\omega_q t + \pi\left(q+\frac{1}{2}\right) + \frac{\phi_G}{2} + \frac{\phi_{r_1}+\phi_{r_2}}{4} - \frac{\phi_G}{2} + \frac{\phi_{r_1}-\phi_{r_2}}{4}\\
=& -\omega_q t + \pi\left(q+\frac{1}{2}\right) + \frac{\phi_{r_2}}{2}
\end{align}

\begin{align}
\Phi_-(z) =& k_q z -\psi(z) - \frac{1}{2}k_q(z_1 + z_2) + \frac{1}{2}(\psi(z_2) + \psi(z_1)) - \frac{\phi_{r_1} - \phi_{r_2}}{4} - \frac{\pi}{2}(q+1)
\end{align}

By plugging in the equation above for $k_q$ (and noting that $L=z_2-z_1$) it can be shown that

\begin{align}
\Phi_-(z_1) =& -\frac{\phi_1}{2} - \pi\left(q+\frac{1}{2}\right) \rightarrow -\frac{\phi_1}{2} \mp \frac{\pi}{2}\\
\Phi_-(z_2) =& \frac{\phi_2}{2} - \frac{\pi}{2}
\end{align}

In the first expression I have replace $\pi q$ by $\pm \pi$ noting that $\mod(\pi q, 2\pi) = \pm \pi$ where the plus sign is taken for even $q$ and the minus sign for odd $q$.

If the cavity is geometrically symmetric then $z_1 = -z_2$ which implies $\psi(z_2) = -\psi(z_1)$ so this simplifies to

\begin{align}
\Phi_- = k_q z - \psi(z) - \frac{\phi_{r_1}-\phi_{r_2}}{4} - \frac{\pi}{2}(q+1)
\end{align}

The total field can then be written as

\begin{align}
E_{cav}(z,t) = 4E_{in,0}^{(+)} t_1\frac{\mathcal{F}}{\pi}\chi(\Delta)&\cos\left(\omega_q t - \pi \left(q+\frac{1}{2}\right) - \frac{\phi_{r_2}}{2}\right)\\
\times&\cos\left(k_qz - \psi(z) - \frac{\phi_{r_1}-\phi_{r_2}}{4} - \frac{\pi}{2}(q+1)\right)
\end{align}





\end{document}