\documentclass[12pt]{article}
\usepackage{amssymb, amsmath, amsfonts}

\usepackage[utf8]{inputenc}
\usepackage{subfigure}%ngerman
\usepackage[pdftex]{graphicx}
\usepackage{textcomp} 
\usepackage{color}
\usepackage[hidelinks]{hyperref}
\usepackage{anysize}
\usepackage{siunitx}
\usepackage{verbatim}
\usepackage{float}
\usepackage{braket}
\usepackage{xfrac}
\usepackage{booktabs}

\usepackage[
sorting=none,
style=numeric
]{biblatex}
\addbibresource{refs.bib}

\newcommand{\ep}{\epsilon}
\newcommand{\sinc}{\text{sinc}}
\newcommand{\bv}[1]{\boldsymbol{#1}}
\newcommand{\ahat}{\hat{a}}
\newcommand{\adag}{\ahat^{\dag}}
\newcommand{\braketacomm}[1]{\left\langle\left\{#1\right\} \right\rangle}
\newcommand{\braketcomm}[1]{\left\langle\left[#1\right] \right\rangle}

\makeatletter
\newcommand{\vast}{\bBigg@{4}}
\newcommand{\Vast}{\bBigg@{5}}
\makeatother


\begin{document}

\begin{align}
&\mathcal{P'}(A_1^1, \ldots, A_1^d, \tau_1 ; \ldots ; A_v^1, \ldots,A_v^d,\tau_v)\\
&= \Braket{\prod_{r=1}^d \prod_{s=1}^v \left(\prod_{k \in A_s^r} y_k \prod_{l \in [N]\setminus A_s^r} (1-y_l) \right)}\\
&= \Braket{\prod_{r=1}^d \prod_{s=1}^v \left( \sum_{j=0}^{N-m_s^r} \frac{(-1)^j}{j!} \sum_{B \in ([N] \setminus A_s^r)_j^P} \prod_{k \in A_s^r \cup B} y_k \right)}\\
&= \vast( \left(\sum_{j_1^1 =0}^{N-m_1^1} \sum_{B_1^1 \in ([N]\setminus A_1^1)_{j_1^1}^P} \frac{(-1)^{j_1^1}}{j_1^1!}
\ldots 
\sum_{j_1^d =0}^{N-m_1^d} \sum_{B_1^d \in ([N]\setminus A_1^d)_{j_1^d}^P} \frac{(-1)^{j_1^d}}{j_1^d!}\right)\\
&\ldots\\
&\left(\sum_{j_v^1 =0}^{N-m_v^1} \sum_{B_v^1 \in ([N]\setminus A_v^1)_{j_v^1}^P} \frac{(-1)^{j_v^1}}{j_v^1!}
\ldots 
\sum_{j_v^d =0}^{N-m_v^d} \sum_{B_v^d \in ([N]\setminus A_v^d)_{j_v^d}^P} \frac{(-1)^{j_v^d}}{j_v^d!} \right) \vast)\\
&\Braket{\prod_{r=1}^d \prod_{s=1}^v \prod_{k \in  A_s^r\cup B_s^r} y_k}\\
&= \vast( \left(\sum_{j_1^1 =0}^{N-m_1^1} \sum_{B_1^1 \in ([N]\setminus A_1^1)_{j_1^1}^P} \frac{(-1)^{j_1^1}}{j_1^1!}
\ldots 
\sum_{j_1^d =0}^{N-m_1^d} \sum_{B_1^d \in ([N]\setminus A_1^d)_{j_1^d}^P} \frac{(-1)^{j_1^d}}{j_1^d!}\right)\\
&\ldots\\
&\left(\sum_{j_v^1 =0}^{N-m_v^1} \sum_{B_v^1 \in ([N]\setminus A_v^1)_{j_v^1}^P} \frac{(-1)^{j_v^1}}{j_v^1!}
\ldots 
\sum_{j_v^d =0}^{N-m_v^d} \sum_{B_v^d \in ([N]\setminus A_v^d)_{j_v^d}^P} \frac{(-1)^{j_v^d}}{j_v^d!} \right) \vast)\\
&\mathcal{P}(A_1^1 \cup B_1^1, \ldots, A_1^d \cup B_1^d, \tau_1 ; \ldots ; A_v^1 \cup B_v^1, \ldots,A_v^d \cup B_v^d,\tau_v)\\
\end{align}


\begin{align}
&P(m_1^1,\ldots,m_1^d,\tau_1; \ldots ; m_v^1, \ldots, m_v^d, \tau_v) =\\
&\left(\left(\sum_{A_1^1 \in ([N])_{m_1^1}^C} \ldots \sum_{A_1^d \in ([N])_{m_1^d}^C}\right) \ldots \left(\sum_{A_v^1 \in ([N])_{m_v^1}^C} \ldots \sum_{A_v^d \in ([N])_{m_v^d}^C}\right)\right)\\
&\mathcal{P'}(A_1^1, \ldots, A_1^d, \tau_1 ; \ldots ; A_v^1, \ldots,A_v^d,\tau_v)\\
&=\left(\left(\sum_{A_1^1 \in ([N])_{m_1^1}^P} \frac{1}{m_1^1!} \ldots \sum_{A_1^d \in ([N])_{m_1^d}^P} \frac{1}{m_1^d!} \right) \ldots \left(\sum_{A_v^1 \in ([N])_{m_v^1}^P} \frac{1}{m_v^1!}  \ldots \sum_{A_v^d \in ([N])_{m_v^d}^P}\frac{1}{m_v^d!} \right)\right)\\
&\mathcal{P'}(A_1^1, \ldots, A_1^d, \tau_1 ; \ldots ; A_v^1, \ldots,A_v^d,\tau_v)\\
&= \vast( \left(\sum_{j_1^1 =0}^{N-m_1^1} \sum_{A_1^1 \in ([N])_{m_1^1}^P} \sum_{B_1^1 \in ([N]\setminus A_1^1)_{j_1^1}^P} \frac{(-1)^{j_1^1}}{m_1^1! j_1^1!}
\ldots 
\sum_{j_1^d =0}^{N-m_1^d}  \sum_{A_1^d \in ([N])_{m_1^d}^P} \sum_{B_1^d \in ([N]\setminus A_1^d)_{j_1^d}^P} \frac{(-1)^{j_1^d}}{m_1^d! j_1^d!}\right)\\
&\ldots\\
&\left(\sum_{j_v^1 =0}^{N-m_v^1}  \sum_{A_v^1 \in ([N])_{m_v^1}^P} \sum_{B_v^1 \in ([N]\setminus A_v^1)_{j_v^1}^P} \frac{(-1)^{j_v^1}}{m_v^1! j_v^1!}
\ldots 
\sum_{j_v^d =0}^{N-m_v^d}  \sum_{A_v^d \in ([N])_{m_v^d}^P} \sum_{B_v^d \in ([N]\setminus A_v^d)_{j_v^d}^P} \frac{(-1)^{j_v^d}}{m_v^d! j_v^d!} \right) \vast)\\
&\mathcal{P}(A_1^1 \cup B_1^1, \ldots, A_1^d \cup B_1^d, \tau_1 ; \ldots ; A_v^1 \cup B_v^1, \ldots,A_v^d \cup B_v^d,\tau_v)\\
&= \vast( \left(\sum_{j_1^1 =0}^{N-m_1^1} \sum_{A_1^1 \in ([N])_{m_1^1+j_1^1}^P} \frac{(-1)^{j_1^1}}{m_1^1! j_1^1!}
\ldots 
\sum_{j_1^d =0}^{N-m_1^d}  \sum_{A_1^d \in ([N])_{m_1^d+j_1^d}^P} \frac{(-1)^{j_1^d}}{m_1^d! j_1^d!}\right)\\
&\ldots\\
&\left(\sum_{j_v^1 =0}^{N-m_v^1}  \sum_{A_v^1 \in ([N])_{m_v^1+j_v^1}^P}  \frac{(-1)^{j_v^1}}{m_v^1! j_v^1!}
\ldots 
\sum_{j_v^d =0}^{N-m_v^d}  \sum_{A_v^d \in ([N])_{m_v^d+j_v^d}^P}  \frac{(-1)^{j_v^d}}{m_v^d! j_v^d!} \right) \vast)\\
&\mathcal{P}(A_1^1, \ldots, A_1^d, \tau_1 ; \ldots ; A_v^1, \ldots,A_v^d,\tau_v)\\
\end{align}

\begin{align}
&\mathcal{P}(A_1^1, \ldots, A_1^d, \tau_1 ; \ldots ; A_v^1, \ldots,A_v^d,\tau_v) =\\
&w(A_1^1, \ldots, A_1^d, \tau_1 ; \ldots ; A_v^1, \ldots,A_v^d,\tau_v) \left((\Delta t)^{m_1^1+j_1^1}\ldots (\Delta t)^{m_1^d+j_1^d} \right) \ldots \left((\Delta t)^{m_v^1+j_v^1}\ldots (\Delta t)^{m_v^d+j_v^d} \right)\\
\end{align}

\begin{align}
&w(A_1^1, \ldots, A_1^d, \tau_1 ; \ldots ; A_v^1, \ldots,A_v^d,\tau_v)\\
&=w\Bigg(t^{(1)}_{i^{(1,1,1)}},\ldots,t^{(1)}_{i^{\left((1,1,m_1^1+j_1^1\right)}} 
;\ldots; t^{(1)}_{i^{(1,d,1)}},\ldots,t^{(1)}_{i^{\left(1,d,m_1^d+j_1^d\right)}}
\big\vert \ldots\\
&\ldots \big\vert
t^{(v)}_{i^{(v,1,1)}},\ldots,t^{(v)}_{i^{\left(v,1,m_v^1+j_v^1\right)}}
;\ldots; t^{(v)}_{i^{(v,d,1)}},\ldots,t^{(v)}_{i^{\left(v,d,m_v^d+j_v^d\right)}}
\Bigg)
\end{align}
	
\begin{align}
&P(m_1^1,\ldots,m_1^d,\tau_1; \ldots ; m_v^1, \ldots, m_v^d, \tau_v) =\\
&\left(\left(\sum_{j_1^1=0}^{N-m_1^1}\frac{(-1)^{j_1^1}}{m_1^1!j_1^1!} 
\ldots \sum_{j_1^d=0}^{N-m_1^d}\frac{(-1)^{j_1^d}}{m_1^d!j_1^d!} \right) 
\ldots
\left(\sum_{j_v^1=0}^{N-m_v^1}\frac{(-1)^{j_v^1}}{m_v^1!j_v^1!} 
\ldots \sum_{j_v^d=0}^{N-m_v^d}\frac{(-1)^{j_v^d}}{m_v^d!j_v^d!} \right) \right)\\
&\vast(\left(\int_{t^{(1,1,1)} = t^{(1)}_0}^{t_0^{(1)}+\Delta T} \ldots \int_{t^{\left(1,1,m_1^1+j_1^1\right)} = t^{(1)}_0}^{t_0^{(1)}+\Delta T}\right) \ldots \left(\int_{t^{(1,d,1)} = t^{(1)}_0}^{t_0^{(1)}+\Delta T} \ldots \int_{t^{\left(1,d,m_1^d+j_1^d\right)} = t^{(1)}_0}^{t_0^{(1)}+\Delta T}\right)\\
&\ldots\\
&\left(\int_{t^{(v,1,1)} = t^{(v)}_0}^{t_0^{(v)}+\Delta T} \ldots \int_{t^{\left(v,1,m_v^1+j_v^1\right)} = t^{(v)}_0}^{t_0^{(v)}+\Delta T}\right) \ldots \left(\int_{t^{(v,d,1)} = t^{(v)}_0}^{t_0^{(v)}+\Delta T} \ldots \int_{t^{\left(v,d, m_v^d+j_v^d\right)} = t^{(v)}_0}^{t_0^{(v)}+\Delta T}\right)\vast)\\
&w\Bigg(t^{(1,1,1)}\ldots t^{\left(1,1,m_1^1+j_1^1\right)};\ldots;t^{(1,d,1)}\ldots t^{\left(1,d,m_1^d+j_1^d\right)}\Big| \ldots\\
&\ldots \Big| t^{(v,1,1)}\ldots t^{\left(v,1,m_v^1+j_v^1\right)};\ldots;t^{(v,d,1)}\ldots t^{\left(v,d,m_v^d+j_v^d\right)}\Bigg)\\
&\left( \left(dt^{(1,1,1)} \ldots dt^{\left(1,1,m_1^1+j_1^1\right)}\right) \ldots \left(dt^{(1,d,1)} \ldots dt^{\left(1,d,m_1^d+j_1^d\right)}\right) \right)\\
&\ldots\\
&\left( \left(dt^{(v,1,1)} \ldots dt^{\left(v,1,m_v^1+j_v^1\right)}\right) \ldots \left(dt^{(v,d,1)} \ldots dt^{\left(v,d,m_v^d+j_v^d\right)}\right) \right)\\
\end{align}	

\begin{align}
&P(m_1^1,\ldots,m_1^d,\tau_1; \ldots ; m_v^1, \ldots, m_v^d, \tau_v) =\\
&\Vast\langle: \left(\left(\sum_{j_1^1=0}^{N-m_1^1}\frac{(-1)^{j_1^1}}{m_1^1!j_1^1!} 
\ldots \sum_{j_1^d=0}^{N-m_1^d}\frac{(-1)^{j_1^d}}{m_1^d!j_1^d!} \right) 
\ldots
\left(\sum_{j_v^1=0}^{N-m_v^1}\frac{(-1)^{j_v^1}}{m_v^1!j_v^1!} 
\ldots \sum_{j_v^d=0}^{N-m_v^d}\frac{(-1)^{j_v^d}}{m_v^d!j_v^d!} \right) \right)\\
&\vast(\left(\int_{t^{(1,1,1)} = t^{(1)}_0}^{t_0^{(1)}+\Delta T} \ldots \int_{t^{\left(1,1,m_1^1+j_1^1\right)} = t^{(1)}_0}^{t_0^{(1)}+\Delta T}\right) \ldots \left(\int_{t^{(1,d,1)} = t^{(1)}_0}^{t_0^{(1)}+\Delta T} \ldots \int_{t^{\left(1,d,m_1^d+j_1^d\right)} = t^{(1)}_0}^{t_0^{(1)}+\Delta T}\right)\\
&\ldots\\
&\left(\int_{t^{(v,1,1)} = t^{(v)}_0}^{t_0^{(v)}+\Delta T} \ldots \int_{t^{\left(v,1,m_v^1+j_v^1\right)} = t^{(v)}_0}^{t_0^{(v)}+\Delta T}\right) \ldots \left(\int_{t^{(v,d,1)} = t^{(v)}_0}^{t_0^{(v)}+\Delta T} \ldots \int_{t^{\left(v,d, m_v^d+j_v^d\right)} = t^{(v)}_0}^{t_0^{(v)}+\Delta T}\right)\vast)\\
&\Bigg(\left(\left(\ep_Q\hat{n}_1(t^{(1,1,1)})\ldots \ep_Q\hat{n}_1(t^{\left(1,1,m_1^1+j_1^1\right)})\right) \ldots \left(\ep_Q\hat{n}_d(t^{(1,d,1)})\ldots \ep_Q\hat{n}_d(t^{\left(1,d,m_1^d+j_1^d\right)})\right)\right)\\
&\ldots \left(\left(\ep_Q \hat{n}_1(t^{(v,1,1)})\ldots \ep_Q\hat{n}_1(t^{\left(v,1,m_v^1+j_v^1\right)})\right) \ldots \left(\ep_Q\hat{n}_d(t^{\left(v,d,1\right)})\ldots \ep_Q\hat{n}_d(t^{\left(v,d,m_v^d+j_v^d\right)})\right)\right)\Bigg)\\
&\left( \left(dt^{(1,1,1)} \ldots dt^{\left(1,1,m_1^1+j_1^1\right)}\right) \ldots \left(dt^{(1,d,1)} \ldots dt^{\left(1,d,m_1^d+j_1^d\right)}\right) \right)\\
&\ldots\\
&\left( \left(dt^{(v,1,1)} \ldots dt^{\left(v,1,m_v^1+j_v^1\right)}\right) \ldots \left(dt^{(v,d,1)} \ldots dt^{\left(v,d,m_v^d+j_v^d\right)}\right) \right):\Vast\rangle\\
\end{align}	

Magically we can factorize the sum under the normal ordering.

\begin{align}
&P(m_1^1,\ldots,m_1^d,\tau_1; \ldots ; m_v^1, \ldots, m_v^d, \tau_v) =\\
&\Vast\langle : 
\left(\sum_{j_1^1=0}^{N-m_1^1}\frac{(-1)^{j_1^1}}{m_1^1!j_1^1!} \left(\ep_Q\int_{t'=t_0^{(1)}}^{t_0^{(1)}+\Delta T}  \hat{n}_1(t') dt'\right)^{m_1^1+j_1^1}
\ldots
\sum_{j_1^d=0}^{N-m_1^d}\frac{(-1)^{j_1^d}}{m_1^d!j_1^d!} \left(\ep_Q\int_{t'=t_0^{(1)}}^{t_0^{(1)}+\Delta T}  \hat{n}_d(t') dt'\right)^{m_1^d+j_1^d}\right)\\
&\ldots\\
&\left(\sum_{j_v^1=0}^{N-m_v^1}\frac{(-1)^{j_v^1}}{m_v^1!j_v^1!} \left(\ep_Q\int_{t'=t_0^{(v)}}^{t_0^{(v)}+\Delta T}  \hat{n}_1(t') dt'\right)^{m_v^1+j_v^1}
\ldots
\sum_{j_v^d=0}^{N-m_v^d}\frac{(-1)^{j_v^d}}{m_v^d!j_v^d!} \left(\ep_Q\int_{t'=t_0^{(v)}}^{t_0^{(v)}+\Delta T}  \hat{n}_d(t') dt'\right)^{m_v^d+j_v^d}\right):\Vast \rangle\\
&= \vast \langle \prod_{r=1}^d \prod_{s=1}^v \sum_{j_s^r=0}^{N-m_s^r}\frac{(-1)^{j_s^r}}{m_s^r!j_s^r!} \left(\ep_Q\int_{t'=t_0^{(s)}}^{t_0^{(s)}+\Delta T} \hat{n}_r(t')dt'\right)^{m_s^r+j_s^r} :\vast\rangle
\end{align}

\begin{align}
\hat{\Omega}_r(t_0^{(q)},t_0^{(q)}+\Delta T) = \ep_Q\int_{t'=t_0^{(q)}}^{t_0^{(q)}+\Delta T}\hat{n}_r(t')dt'
\end{align}

\begin{align}
&P(m_1^1,\ldots,m_1^d,\tau_1; \ldots ; m_v^1, \ldots, m_v^d, \tau_v) =\\
&= \vast \langle : \prod_{r=1}^d \prod_{s=1}^v \sum_{j_s^r=0}^{N-m_s^r}\frac{(-1)^{j_s^r}}{m_s^r!j_s^r!} \left(\hat{\Omega}(t_0^{(s)},t_0^{(s)}+\Delta T)\right)^{m_s^r+j_s^r} :\vast\rangle\\
&= \vast \langle: \prod_{r=1}^d \prod_{s=1}^v \frac{\left(\hat{\Omega}_r(t_0^{(s)},t_0^{(s)}+\Delta T)\right)^{m_s^r}}{m_s^r!} e^{-\hat{\Omega}_r(t_0^{(s)},t_0^{(s)}+\Delta T)} :\vast \rangle
\end{align}
		
\end{document}