\documentclass[12pt]{article}
\usepackage{amssymb, amsmath, amsfonts}

\usepackage[utf8]{inputenc}
\bibliographystyle{plain}
\usepackage{subfigure}%ngerman
\usepackage[pdftex]{graphicx}
\usepackage{textcomp} 
\usepackage{color}
\usepackage[hidelinks]{hyperref}
\usepackage{anysize}
\usepackage{siunitx}
\usepackage{verbatim}
\usepackage{float}
\usepackage{braket}
\usepackage{xfrac}
\usepackage{booktabs}

\newcommand{\ep}{\epsilon}
\newcommand{\sinc}{\text{sinc}}
\newcommand{\bv}[1]{\textbf{#1}}
\newcommand{\ahat}{\hat{a}}
\newcommand{\adag}{\ahat^{\dag}}
\newcommand{\braketacomm}[1]{\left\langle\left\{#1\right\} \right\rangle}
\newcommand{\braketcomm}[1]{\left\langle\left[#1\right] \right\rangle}

\begin{document}
\title{Trig Sum and Difference Forumalas}
\author{Justin Gerber}
\date{\today}
\maketitle

\section{Introduction}

I always forget the trig sum and difference formulas. Maybe writing the identities and their derivations will help me remember them.

\section{Derivation}

\begin{align}
e^{ix} & = \cos(x) + i \sin(x)\\
e^{-ix} &= \cos(x) - i \sin(x)
\end{align}

\begin{align}
\cos(x) &= \frac{1}{2}\left( e^{ix} + e^{-ix}\right)\\
\sin(x) &= \frac{1}{2i}\left( e^{ix} - e^{-ix} \right)
\end{align}

\begin{align}
\cos(x)\cos(y) &= \frac{1}{4} \left(e^{ix} + e^{-ix}\right)\left( e^{iy} + e^{-iy} \right)\\
&=\frac{1}{4}\left( e^{i(x+y)} + e^{-i(x+y)} + e^{i(x-y)} + e^{-i(x-y)}\right)\\
&=\frac{1}{2}\left(\cos(x+y) + \cos(x-y)\right)
\end{align}

\begin{align}
\sin(x)\sin(y) &= -\frac{1}{4} \left(e^{ix} - e^{-ix}\right)\left( e^{iy} - e^{-iy} \right)\\
&=\frac{1}{4}\left( e^{i(x+y)} + e^{-i(x+y)} - e^{i(x-y)} - e^{-i(x-y)}\right)\\
&=-\frac{1}{2}\left(\cos(x+y) - \cos(x-y)\right)
\end{align}

\begin{align}
\cos(x)\sin(y) &= \frac{1}{4i} \left(e^{ix} + e^{-ix}\right)\left( e^{iy} - e^{-iy} \right)\\
&=\frac{1}{4}\left( e^{i(x+y)} - e^{-i(x+y)} - e^{i(x-y)} + e^{-i(x-y)}\right)\\
&=\frac{1}{2}\left(\sin(x+y) - \sin(x-y)\right)
\end{align}

\begin{align}
\sin(x)\cos(y) = \cos(y)\sin(x) &= \frac{1}{2} \left(\sin(y+x) - \sin(y-x)\right)\\
&= \frac{1}{2} \left(\sin(x+y) + \sin(x-y)\right)
\end{align}

\section{Summary}

Product to Sum Formulas:
\begin{align}
\cos(x)\cos(y) &= \frac{1}{2}\left(\cos(x+y) + \cos(x-y)\right)\\
\sin(x)\sin(y) &= -\frac{1}{2}\left(\cos(x+y) - \cos(x-y)\right)\\
\cos(x)\sin(y) &= \frac{1}{2}\left(\sin(x+y) - \sin(x-y)\right)\\
\sin(x)\cos(y) &= \frac{1}{2}\left(\sin(x+y) + \sin(x-y)\right)
\end{align}

Sum to Product Formulas:

\begin{align}
\cos(x+y) &= \cos(x)\cos(y) - \sin(x)\sin(y)\\
\cos(x-y) &= \cos(x)\cos(y) + \sin(x)\sin(y)\\
\sin(x+y) &= \sin(x)\cos(y) + \cos(x)\sin(y)\\
\sin(x-y) &= \sin(x)\cos(y) - \cos(x)\sin(y)
\end{align}

\end{document}